MassageChair/Proofs_R9.thy
@@ -1,0 +1,119 @@
+theory Proofs_R9
+  imports ExtraInv_R9 Requirements
+begin
+
+definition inv9 where "inv9 s \<equiv> extraInv s \<and> R9 s"
+
+theorem "VC1 inv9 s0"
+  apply(unfold VC1_def inv9_def R9_def P6_def)
+  using extra1 VC1_def apply auto
+  done
+
+theorem extra182: "VC182 inv9 env s0 onOff'value startButton'value rollerButton'value vibrationButton'value buttonUp'value buttonDown'value
+ upper'value lower'value"
+  apply(unfold VC182_def inv9_def R9_def)
+  apply(rule impI)
+  apply(rule context_conjI)
+  using extra182 VC182_def apply auto[1]
+apply(rule conjI)
+    apply simp
+  apply(erule conjE)
+     apply(unfold extraInv_def commonExtraInv_def)
+  apply(erule conjE)+
+  apply(rule Pattern6_Def.einv2req1)
+  apply auto
+  done
+
+theorem extra542: "VC542 inv9 env s0 onOff'value startButton'value rollerButton'value vibrationButton'value buttonUp'value buttonDown'value
+ upper'value lower'value"
+  apply(unfold VC542_def inv9_def R9_def)
+  apply(rule impI)
+  apply(rule context_conjI)
+  using extra542 VC542_def apply auto[1]
+apply(rule conjI)
+    apply simp
+  apply(erule conjE)
+     apply(unfold extraInv_def commonExtraInv_def)
+  apply(erule conjE)+
+  apply simp
+  done
+
+theorem extra722: "VC722 inv9 env s0 onOff'value startButton'value rollerButton'value vibrationButton'value buttonUp'value buttonDown'value
+ upper'value lower'value"
+  apply(unfold VC722_def inv9_def R9_def)
+  apply(rule impI)
+  apply(rule context_conjI)
+  using extra722 VC722_def apply auto[1]
+  apply(rule conjI)
+    apply simp
+  apply(erule conjE)
+     apply(unfold extraInv_def commonExtraInv_def)
+  apply(erule conjE)+
+  apply simp
+  apply(rule Pattern6_Def.einv2req1)
+  apply auto
+  done
+
+theorem extra902: "VC902 inv9 env s0 onOff'value startButton'value rollerButton'value vibrationButton'value buttonUp'value buttonDown'value
+ upper'value lower'value"
+  apply(unfold VC902_def inv9_def R9_def)
+  apply(rule impI)
+  apply(rule context_conjI)
+  using extra902 VC902_def apply auto[1]
+  apply(rule conjI)
+    apply simp
+  apply(erule conjE)
+     apply(unfold extraInv_def commonExtraInv_def)
+  apply(erule conjE)+
+  apply simp
+  done
+
+theorem extra1262: "VC1262 inv9 env s0 onOff'value startButton'value rollerButton'value vibrationButton'value buttonUp'value buttonDown'value
+ upper'value lower'value"
+  apply(unfold VC1262_def inv9_def R9_def)
+  apply(rule impI)
+  apply(rule context_conjI)
+  using extra1262 VC1262_def apply auto[1]
+ apply(rule conjI)
+    apply simp
+  apply(erule conjE)
+     apply(unfold extraInv_def commonExtraInv_def)
+  apply(erule conjE)+
+  apply simp
+  apply(rule Pattern6_Def.einv2req1)
+  apply auto
+  done
+
+theorem extra1622: "VC1622 inv9 env s0 onOff'value startButton'value rollerButton'value vibrationButton'value buttonUp'value buttonDown'value
+ upper'value lower'value"
+  apply(unfold VC1622_def inv9_def R9_def)
+  apply(rule impI)
+  apply(rule context_conjI)
+  using extra1622 VC1622_def apply auto[1]
+  apply(rule conjI)
+    apply simp
+  apply(erule conjE)
+     apply(unfold extraInv_def commonExtraInv_def)
+  apply(erule conjE)+
+  apply simp
+  apply(rule Pattern6_Def.einv2req1)
+  apply auto
+  done
+
+theorem extra1802: "VC1802 inv9 env s0 onOff'value startButton'value rollerButton'value vibrationButton'value buttonUp'value buttonDown'value
+ upper'value lower'value"
+  apply(unfold VC1802_def inv9_def R9_def)
+  apply(rule impI)
+  apply(rule context_conjI)
+  using extra1802 VC1802_def apply auto[1]
+  apply(rule conjI)
+    apply simp
+  apply(erule conjE)
+     apply(unfold extraInv_def commonExtraInv_def)
+  apply(erule conjE)+
+  apply simp
+  apply(rule Pattern6_Def.einv2req1)
+  apply auto
+  done
+
+end
