MassageChair/Requirements.thy
@@ -1,31 +1,57 @@
 theory Requirements
-  imports MassageChair
+  imports MassageChair "../Pattern1_Def" "../Pattern6_Def" "../Pattern12_Def" "../Pattern3_Def"
 begin
 
 definition R1 where "R1 s \<equiv> toEnvP s \<and>
 (\<forall> s1. substate s1 s \<and> toEnvP s1 \<and> getVarBool s1 up' = True \<longrightarrow> getVarBool s1 down' = False)"
 
 definition R2 where "R2 s \<equiv> toEnvP s \<and>
-(\<forall> s1. substate s1 s \<and> toEnvP s1 \<and> (getVarBool s1 buttonDown' = False \<or> getVarBool s1 lower' = True) \<longrightarrow> getVarBool s1 down'= True)"
+(\<forall> s1. substate s1 s \<and> toEnvP s1 \<and> (getVarBool s1 buttonDown' = False \<or> getVarBool s1 lower' = True) \<longrightarrow> getVarBool s1 down'= False)"
 
 definition R3 where "R3 s \<equiv> toEnvP s \<and>
-(\<forall> s1 s2. substate s1 s2 \<and> substate s2 s \<and> toEnvP s1 \<and> toEnvP s2 \<and> toEnvNum s1 s2 = 1 \<and>
- getVarBool s1 move' = True \<and> getVarInt s1 vibration' = 0 \<and> getVarBool s2 vibrationButton' = PRESSED' \<and> getVarBool s2 move' = True \<longrightarrow>
- getVarInt s2 vibration' = FAST')"
+(\<forall> s1. substate s1 s \<and> toEnvP s1 \<and> getVarBool s1 enabled' = False \<longrightarrow> getVarBool s1 up' = False \<and> getVarBool s1 down' = False)"
 
 definition R4 where "R4 s \<equiv> toEnvP s \<and>
-(\<forall> s1 s2. substate s1 s2 \<and> substate s2 s \<and> toEnvP s1 \<and> toEnvP s2 \<and> toEnvNum s1 s2 = 1 \<and>
- getVarBool s1 move' = True \<and> getVarInt s1 vibration' = FAST' \<and> getVarBool s2 vibrationButton' = PRESSED' \<and> getVarBool s2 move' = True \<longrightarrow>
- getVarInt s2 vibration' = MODERATE')"
+(\<forall> s2 s1. substate s1 s2 \<and> substate s2 s \<and> toEnvP s1 \<and> toEnvP s2 \<and> toEnvNum s1 s2 = 1 \<and> getVarBool s1 enabled' = False \<and> getVarBool s2 enabled' = True \<and>
+getVarBool s2 rollerButton' = False \<longrightarrow> getVarBool s2 roller' = False)"
 
 definition R5 where "R5 s \<equiv> toEnvP s \<and>
-(\<forall> s1 s2. substate s1 s2 \<and> substate s2 s \<and> toEnvP s1 \<and> toEnvP s2 \<and> toEnvNum s1 s2 = 1 \<and>
- getVarInt s1 vibration' = MODERATE' \<and> getVarBool s2 vibrationButton' = PRESSED' \<longrightarrow>  getVarInt s2 vibration' = 0)"
+(\<forall> s1. substate s1 s \<and> toEnvP s1 \<and> getVarBool s1 rollerButton' = PRESSED' \<and> getVarBool s1 enabled' = True \<longrightarrow> getVarBool s1 roller' = True)"
+
+abbreviation MASSAGE_TIME where "MASSAGE_TIME \<equiv> ROLLER_MASSAGE_TIME'TIMEOUT + VIBRATION_MASSAGE_TIME'TIMEOUT"
 
 definition R6 where "R6 s \<equiv> toEnvP s \<and>
-(\<forall> s1 s2. substate s1 s2 \<and> substate s2 s \<and> toEnvP s1 \<and> toEnvP s2 \<and> toEnvNum s1 s2 = 1 \<and> toEnvNum s2 s \<ge> 20 * 60 * 10 \<and> getVarBool s1 min10' = True \<and>
-getVarBool s2 changeDuration' = PRESSED' \<longrightarrow>
-(\<exists> s4. toEnvP s4 \<and> substate s2 s4 \<and> substate s4 s  \<and> toEnvNum s2 s4 \<le> 20 * 60 *10 \<and> (getVarBool s4 move' = False \<or> getVarBool s4 changeDuration' = PRESSED') \<and>
-(\<forall> s3. toEnvP s3 \<and> substate s2 s3 \<and> substate s3 s4 \<and> s3 \<noteq> s4 \<longrightarrow> getVarBool s3 move' = True \<and> getVarBool s3 changeDuration' = False)))"
+P1 s MASSAGE_TIME (\<lambda> s1. getVarBool s1 roller' = True \<or> getVarBool s1 vibration' = True)
+ (\<lambda> s3. getVarBool s3 roller' = False \<and> getVarBool s3 vibration' = False \<or> getVarBool s3 startButton' = PRESSED')
+(\<lambda> s2. (getVarBool s2 roller' = True \<or> getVarBool s2 vibration' = True) \<and> getVarBool s2 startButton' \<noteq> PRESSED')"
+
+definition R7 where "R7 s \<equiv> toEnvP s \<and>
+(\<forall> s1 s2. substate s1 s2 \<and> substate s2 s \<and> toEnvP s1 \<and> toEnvP s2 \<and> toEnvNum s1 s2 > ON_OFF_TIME'TIMEOUT  \<and> (getVarBool s1 enabled' = True) \<and>
+ (getVarBool s2 onOff' \<noteq> PRESSED') \<and>
+(\<forall>  s3. toEnvP s3 \<and>substate s1 s3 \<and> substate s3 s2 \<and> s1 \<noteq> s3 \<and> s3 \<noteq> s2 \<longrightarrow> getVarBool s3 onOff' = PRESSED') \<longrightarrow>
+getVarBool s2 roller' = False \<and> getVarBool s2 vibration' = False)"
+
+definition R7_1 where "R7_1 s \<equiv> toEnvP s \<and>
+P3 s (\<lambda> s2'.  P12sub s2' ON_OFF_TIME'TIMEOUT (\<lambda> s1. getVarBool s1 enabled' = True) (\<lambda> s2. getVarBool s2 onOff' \<noteq> PRESSED')
+ (\<lambda> s3. getVarBool s3 onOff' = PRESSED'))
+  (\<lambda> s2. getVarBool s2 roller' = False \<and> getVarBool s2 vibration' = False)"
+
+definition R8 where "R8 s \<equiv> toEnvP s \<and>
+(\<forall> s1 s2 s4. substate s1 s2 \<and> substate s2 s4 \<and> substate s4 s \<and> toEnvP s1 \<and> toEnvP s2 \<and> toEnvP s4 \<and> toEnvNum s1 s2 > ON_OFF_TIME'TIMEOUT  \<and> (getVarBool s1 enabled' = True) \<and>
+ (getVarBool s2 onOff' \<noteq> PRESSED') \<and>
+(\<forall>  s3. toEnvP s3 \<and>substate s1 s3 \<and> substate s3 s2 \<and> s1 \<noteq> s3 \<and> s3 \<noteq> s2 \<longrightarrow> getVarBool s3 onOff' = PRESSED') \<and>
+(\<forall> s5. toEnvP s5 \<and> substate s2 s5 \<and> substate s5 s4 \<longrightarrow> getVarBool s5 upper' = False) \<longrightarrow>
+getVarBool s4 up' = True)"
+
+definition R8_1 where "R8_1 s \<equiv> toEnvP s \<and>
+P6_1 s (\<lambda> s2. P12sub s2 ON_OFF_TIME'TIMEOUT (\<lambda> s1. getVarBool s1 enabled' = True) (\<lambda> s2'. getVarBool s2' onOff' \<noteq> PRESSED') (\<lambda> s3. getVarBool s3 onOff' = PRESSED'))
+(\<lambda> s4. getVarBool s4 up' = True)
+(\<lambda> s5. getVarBool s5 upper' = True)"
+
+definition R9 where "R9 s \<equiv> toEnvP s \<and>
+P6 s (\<lambda> s1 s2. getVarBool s1 enabled' = True \<and> getVarBool s2 enabled' = False) (\<lambda> s3. getVarBool s3 up' = True) (\<lambda> s4. getVarBool s4 upper' = True)"
 
 end
+
+
+
