Pattern2_Def.thy
@@ -1,0 +1,27 @@
+theory Pattern2_Def
+  imports Pattern3_Def
+begin
+
+definition P2all where " P2all s A \<equiv>
+\<forall> s1. consecutive s1 s \<longrightarrow> A s1 s"
+
+definition P2ex where "P2ex s A \<equiv>
+\<exists> s1. consecutive s1 s \<and> A s1 s"
+
+definition P2 where  "P2 s A1 A2 \<equiv> toEnvP s \<and>
+(\<forall> s1 s2. consecutive s1 s2 \<and> A1 s1 s2 \<longrightarrow> A2 s1 s2)"
+
+lemma P2all_rule: "consecutive s0 s \<Longrightarrow> P2all s A = A s0 s"
+  apply(unfold consecutive_def P2all_def)
+  by (metis toEnvNum_eq_imp_eq2)
+
+lemma P2ex_rule: "consecutive s0 s \<Longrightarrow> P2ex s A = A s0 s"
+  apply(unfold consecutive_def P2ex_def)
+  by (metis toEnvNum_eq_imp_eq2)
+
+lemma P2_rule: "consecutive s0 s \<Longrightarrow> P2 s0 A1 A2 \<Longrightarrow> (consecutive s0 s \<Longrightarrow> A1 s0 s \<longrightarrow> A2 s0 s) \<Longrightarrow> P2 s A1 A2"
+  apply simp
+  apply(unfold P2_def)
+  using consecutive_def by blast
+
+end
